Moved lemmas to other files, moved general enumeration prefix code to lib

src/travorder/SimIordTraversal.v
@@ -19,50 +19,11 @@ Require Import travorder.IordCoherency.
 Require Import travorder.SimClosure.
 Require Import AuxRel2.
 Require Import ImmFair.
+Require Import EnumPrefix.
 
 Import ListNotations.
 
 Set Implicit Arguments.
-
-(* TODO: move to TLSCoherency *)
-Lemma init_exec_tls_disjoint G:
-  set_disjoint (init_tls G) (exec_tls G). 
-Proof using. unfold init_tls, exec_tls. iord_dom_unfolder. Qed. 
-
-(* TODO: move to SimClosure *)
-Lemma exec_tls_sim_coh G (WF: Wf G):
-  sim_coherent G (exec_tls G).
-Proof using. 
-  unfold sim_coherent, sim_clos. split; [basic_solver| ].
-  repeat (apply set_subset_union_l; split; try basic_solver). 
-  { unfold rmw_clos, exec_tls, tl_covered, tl_issued.
-    repeat rewrite set_pair_alt.
-    rewrite wf_rmwE, wf_rmwD, rmw_non_init_lr; auto. 
-    iord_dom_unfolder; [by vauto| ]. intuition. }
-  { unfold rel_clos, exec_tls, tl_covered, tl_issued.
-    repeat rewrite set_pair_alt.
-    iord_dom_unfolder. left. vauto. }
-Qed.
-
-(* TODO: move to SimClosure*)
-Lemma init_tls_sim_coh G (WF: Wf G):
-  sim_coherent G (init_tls G).
-Proof using. 
-  unfold sim_coherent, sim_clos. split; [basic_solver| ].
-  repeat (apply set_subset_union_l; split); try basic_solver.
-  { unfold rmw_clos. rewrite set_pair_alt. etransitivity.
-    { red. intro. apply proj2. }
-    iord_dom_unfolder. do 2 red in d. desc. red in d. desc.
-    apply init_tls_EI in d. red in d.
-    apply rmw_non_init_lr, seq_eqv_lr in d0; auto. type_solver. }
-  unfold rel_clos. rewrite set_pair_alt. etransitivity.
-  { red. intro. apply proj2. }
-  iord_dom_unfolder. do 2 red in d. desc. red in d. desc.
-  apply init_tls_EI in d. do 2 red in d. desc.
-  destruct y, a0; try by vauto. ins. subst. 
-  forward eapply (wf_init_lab WF l) as ?.
-  unfold is_rel, Events.mod in c. rewrite H in c. vauto. 
-Qed.
 
 Section IordTraversal. 
   Variable (G: execution) (sc: relation actid). 
@@ -112,147 +73,6 @@ Section IordTraversal.
   Notation "'RF'" := (RF G). 
   Notation "'AR'" := (AR G sc). 
   Notation "'FWBOB'" := (FWBOB G).
-
-  Lemma s2tc_coherence_helper WF COMP WFSC CONS
-        (a1 a2: trav_action)
-        (D1 D2: actid -> Prop)
-        (r: relation actid)
-        (S: trav_label -> Prop)
-        (D2R: r ⊆ ⦗D2⦘ ⨾ r)
-        (RELNINIT: r ⊆ r ⨾ ⦗set_compl is_init⦘)
-        (RELE: r ⊆ restr_rel E r)
-        (PREF_CLOS: dom_rel (iord⁺ ;; ⦗S⦘) ⊆₁ S)
-        (REL_IORD: ⦗action ↓₁ eq a2⦘ ⨾ event ↓ r ⨾ ⦗action ↓₁ eq a1⦘ ⊆
-                                     (SB ∪ RF ∪ FWBOB ∪ AR)):
-  dom_rel
-    (r
-     ⨾ ⦗(event ↑₁ (action ↓₁ eq a1 ∩₁ S) ∩₁ D1 \₁ is_init ∪₁ is_init) ∩₁ E⦘)
-    ⊆₁ (event ↑₁ (action ↓₁ eq a2 ∩₁ S) ∩₁ D2 \₁ is_init ∪₁ is_init) ∩₁ E.
-  Proof using.
-    unfolder. intros x [y REL]. desc. des.
-    2: { apply RELNINIT, seq_eqv_r in REL. basic_solver. }
-    destruct y0 as [a y_]. simpl in *. subst a y_.
-    apply RELE in REL. red in REL. desc. clear REL4. splits; auto.
-    destruct (classic (is_init x)); [tauto| left]. splits; auto.
-    2: { apply D2R, seq_eqv_l in REL. basic_solver. } 
-    exists (mkTL a2 x). splits; auto.
-    apply PREF_CLOS. red. eexists. apply seq_eqv_r. split; [| by apply REL5].
-    apply ct_step. do 2 red. splits; try by basic_solver.
-    do 2 left. apply REL_IORD. basic_solver.
-  Qed.
-
-  Section StepsEnum.
-    
-    Variable (steps: nat -> trav_label).
-    Variable (r: relation trav_label).
-    Variable (dom: trav_label -> Prop).
-    Hypothesis (IORD_DOM: r ⊆ dom × dom).
-    Hypothesis (ENUM: enumerates steps dom).
-    Hypothesis (RESP: respects_rel steps r⁺ dom).
-
-    Definition trav_prefix (i: nat) : trav_label -> Prop :=
-      ⋃₁ j < i, eq (steps j).
-
-    Lemma trav_prefix_rel_closed WF COMP WFSC CONS
-          i (DOMi: NOmega.le (NOnum i) (set_size dom)):
-      dom_rel (r⁺ ⨾ ⦗trav_prefix i⦘) ⊆₁ trav_prefix i.
-    Proof using ENUM RESP IORD_DOM.
-      unfold trav_prefix. 
-      red. intros e' [e DOMe']. apply seq_eqv_r in DOMe' as [REL ENUMe].
-      red in ENUMe. destruct ENUMe as [j [LTji STEPje]].
-      apply enumeratesE' in ENUM. cdes ENUM.
-      specialize (IND e'). specialize_full IND.
-      { eapply clos_trans_more in REL.
-        2: { symmetry. apply dom_helper_3. eauto. }
-        apply ct_begin in REL. generalize REL. clear. basic_solver. }
-        
-      destruct IND as [k [DOMk STEPke']].
-      red. exists k. splits; eauto.      
-      etransitivity; [| apply LTji].
-      red in RESP. apply RESP with (j := j); eauto.
-      2: congruence.
-      liaW (set_size dom). 
-    Qed. 
-
-    (* TODO: generalize to arbitrary enumerations? *)
-    Lemma prefix_border i (DOMi: NOmega.lt_nat_l i (set_size dom)):
-      ~ trav_prefix i (steps i).
-    Proof using ENUM.
-      unfold trav_prefix. intros [j [LT EQ]]. 
-      apply enumeratesE' in ENUM. cdes ENUM.
-      forward eapply INJ; [| | apply EQ| lia]; auto. 
-      eapply NOmega.lt_lt_nat; eauto.
-    Qed.
-
-    (* Lemma step_event_dom i (DOMi: NOmega.lt_nat_l i (set_size dom)): *)
-    (*   (E \₁ is_init) (event (steps i)) /\ *)
-    (*   (action (steps i) = ta_issue -> W (event (steps i))).  *)
-    (* Proof using ENUM.  *)
-    (*   apply enumeratesE' in ENUM. cdes ENUM. *)
-    (*   specialize_full INSET; eauto. red in INSET. *)
-    (*   destruct (steps i) as [a e]. unfolder in INSET. basic_solver.  *)
-    (* Qed.  *)
-    Lemma step_event_dom i (DOMi: NOmega.lt_nat_l i (set_size dom)):
-      dom (steps i). 
-    Proof using ENUM.
-      apply enumeratesE' in ENUM. cdes ENUM.
-      specialize_full INSET; eauto. 
-    Qed.       
-
-    Lemma trav_prefix_ext i
-          (DOMi: NOmega.lt_nat_l i (set_size dom)):
-      trav_prefix (S i) ≡₁ trav_prefix i ∪₁ eq (steps i).
-    Proof using. 
-      unfold trav_prefix.
-      arewrite ((fun x => x < S i) ≡₁ (fun x => x < i) ∪₁ eq i).
-      { unfolder. split; ins; lia. }
-      rewrite set_bunion_union_l. basic_solver.
-    Qed.
-
-  Lemma trav_prefix_init:
-    trav_prefix 0 ≡₁ ∅. 
-  Proof using.
-    unfold trav_prefix. apply set_subset_empty_r, set_subset_bunion_l.
-    ins. lia. 
-  Qed.
-  
-  Lemma trav_prefix_r_closed 
-        (i : nat) (DOMi: NOmega.le (NOnum i) (set_size dom)):
-    dom_rel (r ⨾ ⦗trav_prefix i⦘) ⊆₁ trav_prefix i.
-  Proof using RESP ENUM IORD_DOM.
-    induction i.
-    { rewrite trav_prefix_init. red. basic_solver. }
-    rewrite trav_prefix_ext; eauto. 
-    rewrite id_union, seq_union_r, dom_union.
-    apply set_subset_union_l. split. 
-    { unfold iord_coherent in IHi. rewrite IHi; [basic_solver| ].
-      liaW (set_size dom). }
-    red. intros tlj. intros [tli IORD%seq_eqv_r]. desc.
-    (* apply iord_exec_tls in IORD. red in IORD. desc. *)
-    apply dom_helper_3 in IORD_DOM.
-    apply IORD_DOM, seq_eqv_lr in IORD as (Dj & Rji & Di).  
-    apply enumeratesE' in ENUM. cdes ENUM.
-    apply IND in Dj, Di. desc. rename i1 into j.
-    assert (i0 = i) as -> by (apply INJ; auto; congruence).
-    subst. 
-    pose proof (Nat.lt_trichotomy i j) as LT. des; revgoals. 
-    { left. red. vauto. }
-    { subst. basic_solver. }
-    (* TODO: is the last tactic needed? *)
-    enough (j < i); [lia| ]. eapply RESP; eauto; try by apply ct_step.
-  Qed.
-  
-  Lemma trav_prefix_in_dom i
-        (DOMi: NOmega.le (NOnum i) (set_size dom)):
-    trav_prefix i ⊆₁ dom. 
-  Proof using ENUM. 
-    apply enumeratesE' in ENUM. cdes ENUM. 
-    unfold trav_prefix. apply set_subset_bunion_l. intros.
-    apply set_subset_single_l. apply INSET.
-    liaW (set_size dom). 
-  Qed.
-
-  End StepsEnum.
 
   Section IordEnum.
     (* This generalization is used to support traversal 
@@ -352,12 +172,9 @@ Section IordTraversal.
 
   End IordEnum. 
 
-
   Lemma iord_enum_exists WF COMP WFSC CONS MF
         (IMM_FAIR: imm_s_fair G sc)
-        dom
-        (* (IORD_DOM: iord ⊆ dom × dom) (DOM_EXEC: dom ⊆₁ exec_tls G) *)
-    :
+        dom:
   exists (steps: nat -> trav_label),
     enumerates steps dom /\
     respects_rel steps iord⁺ dom. 
@@ -380,8 +197,6 @@ Section IordTraversal.
     apply ct_begin in Rij. generalize Rij. unfold iord. basic_solver. 
   Qed.
 
-
-  (* TODO: rename? *)
   Lemma sim_traversal_inf WF CONS
         (FAIR: mem_fair G)
         (IMM_FAIR: imm_s_fair G sc)
@@ -423,78 +238,6 @@ Section IordTraversal.
     eapply trav_prefix_in_dom; eauto.
   Qed.
 
-  Lemma exec_tls_cip_alt:
-    exec_tls_cip G ≡₁ exec_tls G \₁ action ↓₁ eq ta_reserve. 
-  Proof using. 
-    unfold exec_tls_cip, exec_tls. rewrite !set_pair_alt.
-    split; try basic_solver 10.
-    rewrite set_minus_union_l.
-    unfolder. ins. destruct x; ins; des; subst; splits; try by vauto.
-    { right. splits; vauto. }
-    do 2 red in H. desc. subst. right. splits; vauto. 
-  Qed. 
-
-  (* TODO: move *)
-  Lemma iord_exec_tls_cip:
-    iord ⊆ exec_tls_cip G × exec_tls_cip G. 
-  Proof using.
-    rewrite exec_tls_cip_alt, set_minusE.
-    rewrite restr_rel_cross_inter.
-    split.
-    { eapply iord_exec_tls; eauto. }
-    do 2 red in H. desc. clear -H. unfolder in H. des.
-    all: apply seq_eqv_lr in H as (X & _ & Y); red in X, Y; vauto;
-      split; red; intros [=]; try congruence.
-    { do 2 red in Y. desc. congruence. }
-    { do 2 red in Y. desc. congruence. } 
-  Qed. 
-
-  Lemma rmw_clos_exec_tls tc (WF: Wf G):
-    rmw_clos G tc ⊆₁ exec_tls G. 
-  Proof using.
-    unfold rmw_clos, exec_tls. rewrite !set_pair_alt.
-    arewrite (codom_rel (⦗tl_covered tc⦘ ⨾ rmw) ⊆₁ (E \₁ is_init) ∩₁ W).
-    2: { basic_solver 10. }
-    rewrite wf_rmwD, wf_rmwE, rmw_in_sb, no_sb_to_init; auto. basic_solver.
-  Qed. 
-  
-  Lemma rel_clos_exec_tls tc (WF: Wf G) (TC_E: tc ⊆₁ event ↓₁ E):
-    rel_clos G tc ⊆₁ exec_tls G.
-  Proof using.
-    unfold rel_clos, exec_tls. rewrite !set_pair_alt.
-    apply set_subset_union_r. left. apply set_subset_inter; [done| ].
-    apply set_map_mori; [done| ]. unfold tl_issued.
-    unfolder. ins. desc. split.
-    { apply TC_E in H0. vauto. }
-    eintros INIT%init_pln; eauto. mode_solver.
-  Qed.
-  
-  Lemma sim_clos_exec_tls WF tc
-        (TC_EXEC: tc ⊆₁ exec_tls G):
-    sim_clos G tc ⊆₁ exec_tls G. 
-  Proof using.
-    repeat (apply set_subset_union_l; split); auto.
-    { by apply rmw_clos_exec_tls. }
-    apply rel_clos_exec_tls; auto. rewrite TC_EXEC.
-    rewrite exec_tls_ENI. basic_solver. 
-  Qed.
-  
-  (* TODO: replace original proof with this + lemmas above *)
-  Lemma sim_clos_tls_coherent' WF tc
-        (TCOH: tls_coherent G tc):
-    tls_coherent G (sim_clos G tc). 
-  Proof using.
-    pose proof TCOH as TCOH'.
-    apply tls_coherent_defs_equiv. apply tls_coherent_defs_equiv in TCOH.
-    red in TCOH. desc.
-    red. unfold sim_clos. exists (tc' ∪₁ rmw_clos G tc ∪₁ rel_clos G tc). split.
-    2: { rewrite TCOH0 at 1. basic_solver. }
-    repeat (apply set_subset_union_l; split); auto.
-    { by apply rmw_clos_exec_tls. }
-    apply rel_clos_exec_tls; auto. by apply tlsc_E. 
-  Qed.  
-
-  (* TODO: rename? *)
   Lemma sim_traversal_inf_cip WF CONS
         (FAIR: mem_fair G)
         (IMM_FAIR: imm_s_fair G sc)
@@ -512,7 +255,7 @@ Section IordTraversal.
           sim_enum i ⊆₁ init_tls G ∪₁ exec_tls_cip G⟫.
   Proof using.
     forward eapply sim_traversal_inf with (dom := exec_tls_cip G) as TRAV; eauto.
-    { apply iord_exec_tls_cip. }
+    { apply dom_helper_3. rewrite <- restr_relE. apply iord_exec_tls_cip. }
     { unfold exec_tls_cip, exec_tls. rewrite !set_pair_alt. basic_solver 10. }
     { unfold exec_tls_cip, exec_tls. rewrite !set_pair_alt. basic_solver 10. }
     ins. rewrite exec_tls_cip_alt, set_minusE. apply set_subset_inter_r. split.
@@ -523,7 +266,6 @@ Section IordTraversal.
     rewrite S_DOM, exec_tls_cip_alt. basic_solver. 
   Qed.
 
-  (* TODO: rename? *)
   Lemma sim_traversal_inf_full WF CONS
         (FAIR: mem_fair G)
         (IMM_FAIR: imm_s_fair G sc):
