src/lib/EnumPrefix.v
@@ -1,0 +1,106 @@
+From hahn Require Import Hahn.
+Require Import AuxRel2.
+Require Import AuxDef. 
+Require Import SetSize. 
+Require Import Lia. 
+
+Section EnumPrefix.
+Context {A: Type}. 
+Variable (steps: nat -> A).
+Variable (r: relation A).
+Variable (dom: A -> Prop).
+Hypothesis (R_DOM: r ⊆ dom × dom).
+Hypothesis (ENUM: enumerates steps dom).
+Hypothesis (RESP: respects_rel steps r⁺ dom).
+
+Definition trav_prefix (i: nat) : A -> Prop :=
+  ⋃₁ j < i, eq (steps j).
+
+Lemma trav_prefix_rel_closed i (DOMi: NOmega.le (NOnum i) (set_size dom)):
+  dom_rel (r⁺ ⨾ ⦗trav_prefix i⦘) ⊆₁ trav_prefix i.
+Proof using ENUM RESP R_DOM.
+  unfold trav_prefix. 
+  red. intros e' [e DOMe']. apply seq_eqv_r in DOMe' as [REL ENUMe].
+  red in ENUMe. destruct ENUMe as [j [LTji STEPje]].
+  apply enumeratesE' in ENUM. cdes ENUM.
+  specialize (IND e'). specialize_full IND.
+  { eapply clos_trans_more in REL.
+    2: { symmetry. apply dom_helper_3. eauto. }
+    apply ct_begin in REL. generalize REL. clear. basic_solver. }
+  
+  destruct IND as [k [DOMk STEPke']].
+  red. exists k. splits; eauto.      
+  etransitivity; [| apply LTji].
+  red in RESP. apply RESP with (j := j); eauto.
+  2: congruence.
+  liaW (set_size dom). 
+Qed. 
+
+Lemma prefix_border i (DOMi: NOmega.lt_nat_l i (set_size dom)):
+  ~ trav_prefix i (steps i).
+Proof using ENUM.
+  unfold trav_prefix. intros [j [LT EQ]]. 
+  apply enumeratesE' in ENUM. cdes ENUM.
+  forward eapply INJ; [| | apply EQ| lia]; auto. 
+  eapply NOmega.lt_lt_nat; eauto.
+Qed.
+
+Lemma step_event_dom i (DOMi: NOmega.lt_nat_l i (set_size dom)):
+  dom (steps i). 
+Proof using ENUM.
+  apply enumeratesE' in ENUM. cdes ENUM.
+  specialize_full INSET; eauto. 
+Qed.       
+
+Lemma trav_prefix_ext i
+      (DOMi: NOmega.lt_nat_l i (set_size dom)):
+  trav_prefix (S i) ≡₁ trav_prefix i ∪₁ eq (steps i).
+Proof using. 
+  unfold trav_prefix.
+  arewrite ((fun x => x < S i) ≡₁ (fun x => x < i) ∪₁ eq i).
+  { unfolder. split; ins; lia. }
+  rewrite set_bunion_union_l. basic_solver.
+Qed.
+
+Lemma trav_prefix_init:
+  trav_prefix 0 ≡₁ ∅. 
+Proof using.
+  unfold trav_prefix. apply set_subset_empty_r, set_subset_bunion_l.
+  ins. lia. 
+Qed.
+
+Lemma trav_prefix_r_closed 
+      (i : nat) (DOMi: NOmega.le (NOnum i) (set_size dom)):
+  dom_rel (r ⨾ ⦗trav_prefix i⦘) ⊆₁ trav_prefix i.
+Proof using RESP ENUM R_DOM.
+  induction i.
+  { rewrite trav_prefix_init. red. basic_solver. }
+  rewrite trav_prefix_ext; eauto. 
+  rewrite id_union, seq_union_r, dom_union.
+  apply set_subset_union_l. split. 
+  { rewrite IHi; [basic_solver| ]. liaW (set_size dom). }
+  red. intros tlj. intros [tli R%seq_eqv_r]. desc.
+  apply dom_helper_3 in R_DOM.
+  apply R_DOM, seq_eqv_lr in R as (Dj & Rji & Di).  
+  apply enumeratesE' in ENUM. cdes ENUM.
+  apply IND in Dj, Di. desc. rename i1 into j.
+  assert (i0 = i) as -> by (apply INJ; auto; congruence).
+  subst. 
+  pose proof (NPeano.Nat.lt_total i j) as LT. des; revgoals. 
+  { left. red. vauto. }
+  { subst. basic_solver. }
+  (* TODO: is the last tactic needed? *)
+  enough (j < i); [lia| ]. eapply RESP; eauto; try by apply ct_step.
+Qed.
+
+Lemma trav_prefix_in_dom i
+      (DOMi: NOmega.le (NOnum i) (set_size dom)):
+  trav_prefix i ⊆₁ dom. 
+Proof using ENUM. 
+  apply enumeratesE' in ENUM. cdes ENUM. 
+  unfold trav_prefix. apply set_subset_bunion_l. intros.
+  apply set_subset_single_l. apply INSET.
+  liaW (set_size dom). 
+Qed.
+
+End EnumPrefix.
